wip

src/Init/WFExtrinsicFix.lean
@@ -30,6 +30,7 @@ variable {α : Sort _} {β : α → Sort _} {γ : (a : α) → β a → Sort _}
 set_option doc.verso true
 
 namespace WellFounded
+open Relation
 
 /--
 The function implemented as the loop {lean}`opaqueFix R F a = F a (fun a _ => opaqueFix R F a)`.
@@ -53,49 +54,49 @@ A fixpoint combinator that can be used to construct recursive functions with an 
 of termination.
 
 Given a relation {name}`R` and a fixpoint functional {name}`F` which must be decreasing with respect
-to {name}`R`, {lean}`extrinsicFix R F` is the recursive function obtained by having {name}`F` call
+to {name}`R`, {lean}`totalExtrinsicFix R F` is the recursive function obtained by having {name}`F` call
 itself recursively.
 
-If {name}`R` is not well-founded, {lean}`extrinsicFix R F` might run forever. In this case,
+If {name}`R` is not well-founded, {lean}`totalExtrinsicFix R F` might run forever. In this case,
 nothing interesting can be proved about the recursive function; it is opaque.
 
-If {name}`R` _is_ well-founded, {lean}`extrinsicFix R F` is equivalent to
+If {name}`R` _is_ well-founded, {lean}`totalExtrinsicFix R F` is equivalent to
 {lean}`WellFounded.fix _ F`, logically and regarding its termination behavior.
 -/
 @[implemented_by opaqueFix]
-public def extrinsicFix [∀ a, Nonempty (C a)] (R : α → α → Prop)
+public def totalExtrinsicFix [∀ a, Nonempty (C a)] (R : α → α → Prop)
     (F : ∀ a, (∀ a', R a' a → C a') → C a) (a : α) : C a :=
   open scoped Classical in
   if h : WellFounded R then
     h.fix F a
   else
     -- Return `opaqueFix R F a` so that `implemented_by opaqueFix` is sound.
-    -- In effect, `extrinsicFix` is opaque if `WellFounded R` is false.
+    -- In effect, `totalExtrinsicFix` is opaque if `WellFounded R` is false.
     opaqueFix R F a
 
-public theorem extrinsicFix_eq_fix [∀ a, Nonempty (C a)] {R : α → α → Prop}
+public theorem totalExtrinsicFix_eq_fix [∀ a, Nonempty (C a)] {R : α → α → Prop}
     {F : ∀ a, (∀ a', R a' a → C a') → C a}
     (wf : WellFounded R) {a : α} :
-    extrinsicFix R F a = wf.fix F a := by
-  simp only [extrinsicFix, dif_pos wf]
+    totalExtrinsicFix R F a = wf.fix F a := by
+  simp only [totalExtrinsicFix, dif_pos wf]
 
-public theorem extrinsicFix_eq_apply [∀ a, Nonempty (C a)] {R : α → α → Prop}
+public theorem totalExtrinsicFix_eq_apply [∀ a, Nonempty (C a)] {R : α → α → Prop}
     {F : ∀ a, (∀ a', R a' a → C a') → C a} (h : WellFounded R) {a : α} :
-    extrinsicFix R F a = F a (fun a _ => extrinsicFix R F a) := by
-  simp only [extrinsicFix, dif_pos h]
+    totalExtrinsicFix R F a = F a (fun a _ => totalExtrinsicFix R F a) := by
+  simp only [totalExtrinsicFix, dif_pos h]
   rw [WellFounded.fix_eq]
 
 /--
 A fixpoint combinator that allows for deferred proofs of termination.
 
-{lean}`extrinsicFix R F` is function implemented as the loop
-{lean}`extrinsicFix R F a = F a (fun a _ => extrinsicFix R F a)`.
+{lean}`totalExtrinsicFix R F` is function implemented as the loop
+{lean}`totalExtrinsicFix R F a = F a (fun a _ => totalExtrinsicFix R F a)`.
 
-If the loop can be shown to be well-founded, {name}`extrinsicFix_eq_apply` proves that it satisfies the
-fixpoint equation. Otherwise, {lean}`extrinsicFix R F` is opaque, i.e., it is impossible to prove
+If the loop can be shown to be well-founded, {name}`totalExtrinsicFix_eq_apply` proves that it satisfies the
+fixpoint equation. Otherwise, {lean}`totalExtrinsicFix R F` is opaque, i.e., it is impossible to prove
 nontrivial properties about it.
 -/
-add_decl_doc extrinsicFix
+add_decl_doc totalExtrinsicFix
 
 /--
 The function implemented as the loop
@@ -123,51 +124,51 @@ A fixpoint combinator that can be used to construct recursive functions of arity
 *extrinsic* proof of termination.
 
 Given a relation {name}`R` and a fixpoint functional {name}`F` which must be decreasing with respect
-to {name}`R`, {lean}`extrinsicFix₂ R F` is the recursive function obtained by having {name}`F` call
+to {name}`R`, {lean}`totalExtrinsicFix₂ R F` is the recursive function obtained by having {name}`F` call
 itself recursively.
 
-If {name}`R` is not well-founded, {lean}`extrinsicFix₂ R F` might run forever. In this case,
+If {name}`R` is not well-founded, {lean}`totalExtrinsicFix₂ R F` might run forever. In this case,
 nothing interesting can be proved about the recursive function; it is opaque.
 
-If {name}`R` _is_ well-founded, {lean}`extrinsicFix₂ R F` is equivalent to a well-founded recursive
+If {name}`R` _is_ well-founded, {lean}`totalExtrinsicFix₂ R F` is equivalent to a well-founded recursive
 function, logically and regarding its termination behavior.
 -/
 @[implemented_by opaqueFix₂]
-public def extrinsicFix₂ [∀ a b, Nonempty (C₂ a b)]
+public def totalExtrinsicFix₂ [∀ a b, Nonempty (C₂ a b)]
     (R : (a : α) ×' β a → (a : α) ×' β a → Prop)
     (F : (a : α) → (b : β a) → ((a' : α) → (b' : β a') → R ⟨a', b'⟩ ⟨a, b⟩ → C₂ a' b') → C₂ a b)
     (a : α) (b : β a) :
     C₂ a b :=
   let F' (x : PSigma β) (G : (y : PSigma β) → R y x → C₂ y.1 y.2) : C₂ x.1 x.2 :=
     F x.1 x.2 (fun a b => G ⟨a, b⟩)
-  extrinsicFix (C := fun x : PSigma β => C₂ x.1 x.2) R F' ⟨a, b⟩
+  totalExtrinsicFix (C := fun x : PSigma β => C₂ x.1 x.2) R F' ⟨a, b⟩
 
-public theorem extrinsicFix₂_eq_fix [∀ a b, Nonempty (C₂ a b)]
+public theorem totalExtrinsicFix₂_eq_fix [∀ a b, Nonempty (C₂ a b)]
     {R : (a : α) ×' β a → (a : α) ×' β a → Prop}
     {F : ∀ a b, (∀ a' b', R ⟨a', b'⟩ ⟨a, b⟩ → C₂ a' b') → C₂ a b}
     (wf : WellFounded R) {a b} :
-    extrinsicFix₂ R F a b = wf.fix (fun x G => F x.1 x.2 (fun a b h => G ⟨a, b⟩ h)) ⟨a, b⟩ := by
-  rw [extrinsicFix₂, extrinsicFix_eq_fix wf]
+    totalExtrinsicFix₂ R F a b = wf.fix (fun x G => F x.1 x.2 (fun a b h => G ⟨a, b⟩ h)) ⟨a, b⟩ := by
+  rw [totalExtrinsicFix₂, totalExtrinsicFix_eq_fix wf]
 
-public theorem extrinsicFix₂_eq_apply [∀ a b, Nonempty (C₂ a b)]
+public theorem totalExtrinsicFix₂_eq_apply [∀ a b, Nonempty (C₂ a b)]
     {R : (a : α) ×' β a → (a : α) ×' β a → Prop}
     {F : (a : α) → (b : β a) → ((a' : α) → (b' : β a') → R ⟨a', b'⟩ ⟨a, b⟩ → C₂ a' b') → C₂ a b}
     (wf : WellFounded R) {a : α} {b : β a} :
-    extrinsicFix₂ R F a b = F a b (fun a' b' _ => extrinsicFix₂ R F a' b') := by
-  rw [extrinsicFix₂, extrinsicFix_eq_apply wf]
+    totalExtrinsicFix₂ R F a b = F a b (fun a' b' _ => totalExtrinsicFix₂ R F a' b') := by
+  rw [totalExtrinsicFix₂, totalExtrinsicFix_eq_apply wf]
   rfl
 
 /--
 A fixpoint combinator that allows for deferred proofs of termination.
 
-{lean}`extrinsicFix₂ R F` is function implemented as the loop
-{lean}`extrinsicFix₂ R F a b = F a b (fun a' b' _ => extrinsicFix₂ R F a' b')`.
+{lean}`totalExtrinsicFix₂ R F` is function implemented as the loop
+{lean}`totalExtrinsicFix₂ R F a b = F a b (fun a' b' _ => totalExtrinsicFix₂ R F a' b')`.
 
-If the loop can be shown to be well-founded, {name}`extrinsicFix₂_eq_apply` proves that it satisfies the
-fixpoint equation. Otherwise, {lean}`extrinsicFix₂ R F` is opaque, i.e., it is impossible to prove
+If the loop can be shown to be well-founded, {name}`totalExtrinsicFix₂_eq_apply` proves that it satisfies the
+fixpoint equation. Otherwise, {lean}`totalExtrinsicFix₂ R F` is opaque, i.e., it is impossible to prove
 nontrivial properties about it.
 -/
-add_decl_doc extrinsicFix₂
+add_decl_doc totalExtrinsicFix₂
 
 /--
 The function implemented as the loop
@@ -195,17 +196,17 @@ A fixpoint combinator that can be used to construct recursive functions of arity
 *extrinsic* proof of termination.
 
 Given a relation {name}`R` and a fixpoint functional {name}`F` which must be decreasing with respect
-to {name}`R`, {lean}`extrinsicFix₃ R F` is the recursive function obtained by having {name}`F` call
+to {name}`R`, {lean}`totalExtrinsicFix₃ R F` is the recursive function obtained by having {name}`F` call
 itself recursively.
 
-If {name}`R` is not well-founded, {lean}`extrinsicFix₃ R F` might run forever. In this case,
+If {name}`R` is not well-founded, {lean}`totalExtrinsicFix₃ R F` might run forever. In this case,
 nothing interesting can be proved about the recursive function; it is opaque.
 
-If {name}`R` _is_ well-founded, {lean}`extrinsicFix₃ R F` is equivalent to a well-founded recursive
+If {name}`R` _is_ well-founded, {lean}`totalExtrinsicFix₃ R F` is equivalent to a well-founded recursive
 function, logically and regarding its termination behavior.
 -/
 @[implemented_by opaqueFix₃]
-public def extrinsicFix₃ [∀ a b c, Nonempty (C₃ a b c)]
+public def totalExtrinsicFix₃ [∀ a b c, Nonempty (C₃ a b c)]
     (R : (a : α) ×' (b : β a) ×' γ a b → (a : α) ×' (b : β a) ×' γ a b → Prop)
     (F : ∀ (a b c), (∀ (a' b' c'), R ⟨a', b', c'⟩ ⟨a, b, c⟩ → C₃ a' b' c') → C₃ a b c)
     (a : α) (b : β a) (c : γ a b) :
@@ -213,33 +214,192 @@ public def extrinsicFix₃ [∀ a b c, Nonempty (C₃ a b c)]
   let F' (x : (a : α) ×' (b : β a) ×' γ a b) (G : (y : (a : α) ×' (b : β a) ×' γ a b) → R y x → C₃ y.1 y.2.1 y.2.2) :
       C₃ x.1 x.2.1 x.2.2 :=
     F x.1 x.2.1 x.2.2 (fun a b c => G ⟨a, b, c⟩)
-  extrinsicFix (C := fun x : (a : α) ×' (b : β a) ×' γ a b => C₃ x.1 x.2.1 x.2.2) R F' ⟨a, b, c⟩
+  totalExtrinsicFix (C := fun x : (a : α) ×' (b : β a) ×' γ a b => C₃ x.1 x.2.1 x.2.2) R F' ⟨a, b, c⟩
 
-public theorem extrinsicFix₃_eq_fix [∀ a b c, Nonempty (C₃ a b c)]
+public theorem totalExtrinsicFix₃_eq_fix [∀ a b c, Nonempty (C₃ a b c)]
     {R : (a : α) ×' (b : β a) ×' γ a b → (a : α) ×' (b : β a) ×' γ a b → Prop}
     {F : ∀ a b c, (∀ a' b' c', R ⟨a', b', c'⟩ ⟨a, b, c⟩ → C₃ a' b' c') → C₃ a b c}
     (wf : WellFounded R) {a b c} :
-    extrinsicFix₃ R F a b c = wf.fix (fun x G => F x.1 x.2.1 x.2.2 (fun a b c h => G ⟨a, b, c⟩ h)) ⟨a, b, c⟩ := by
-  rw [extrinsicFix₃, extrinsicFix_eq_fix wf]
+    totalExtrinsicFix₃ R F a b c = wf.fix (fun x G => F x.1 x.2.1 x.2.2 (fun a b c h => G ⟨a, b, c⟩ h)) ⟨a, b, c⟩ := by
+  rw [totalExtrinsicFix₃, totalExtrinsicFix_eq_fix wf]
 
-public theorem extrinsicFix₃_eq_apply [∀ a b c, Nonempty (C₃ a b c)]
+public theorem totalExtrinsicFix₃_eq_apply [∀ a b c, Nonempty (C₃ a b c)]
     {R : (a : α) ×' (b : β a) ×' γ a b → (a : α) ×' (b : β a) ×' γ a b → Prop}
     {F : ∀ (a b c), (∀ (a' b' c'), R ⟨a', b', c'⟩ ⟨a, b, c⟩ → C₃ a' b' c') → C₃ a b c}
     (wf : WellFounded R) {a : α} {b : β a} {c : γ a b} :
-    extrinsicFix₃ R F a b c = F a b c (fun a b c _ => extrinsicFix₃ R F a b c) := by
-  rw [extrinsicFix₃, extrinsicFix_eq_apply wf]
+    totalExtrinsicFix₃ R F a b c = F a b c (fun a b c _ => totalExtrinsicFix₃ R F a b c) := by
+  rw [totalExtrinsicFix₃, totalExtrinsicFix_eq_apply wf]
   rfl
 
 /--
 A fixpoint combinator that allows for deferred proofs of termination.
 
-{lean}`extrinsicFix₃ R F` is function implemented as the loop
-{lean}`extrinsicFix₃ R F a b c = F a b c (fun a b c _ => extrinsicFix₃ R F a b c)`.
+{lean}`totalExtrinsicFix₃ R F` is function implemented as the loop
+{lean}`totalExtrinsicFix₃ R F a b c = F a b c (fun a b c _ => totalExtrinsicFix₃ R F a b c)`.
 
-If the loop can be shown to be well-founded, {name}`extrinsicFix₃_eq_apply` proves that it satisfies the
-fixpoint equation. Otherwise, {lean}`extrinsicFix₃ R F` is opaque, i.e., it is impossible to prove
+If the loop can be shown to be well-founded, {name}`totalExtrinsicFix₃_eq_apply` proves that it satisfies the
+fixpoint equation. Otherwise, {lean}`totalExtrinsicFix₃ R F` is opaque, i.e., it is impossible to prove
 nontrivial properties about it.
 -/
-add_decl_doc extrinsicFix₃
+add_decl_doc totalExtrinsicFix₃
+
+@[inline]
+public def WellFounded.extrinsicFix [∀ a, Nonempty (C a)] (R : α → α → Prop)
+    (F : ∀ a, (∀ a', R a' a → C a') → C a) (a : α) : C a :=
+  totalExtrinsicFix (α := { a' : α // a' = a ∨ TransGen R a' a }) (C := (C ·.1))
+      (fun p q => R p.1 q.1)
+      (fun a recur => F a.1 fun a' hR => recur ⟨a', by
+        rcases a.property with ha | ha
+        · exact Or.inr (TransGen.single (ha ▸ hR))
+        · apply Or.inr
+          apply TransGen.trans ?_ ‹_›
+          apply TransGen.single
+          assumption⟩ ‹_›) ⟨a, Or.inl rfl⟩
+
+public theorem WellFounded.totalExtrinsicFix_invImage {α' : Sort _} [∀ a, Nonempty (C a)] (R : α → α → Prop) (f : α' → α)
+    (F : ∀ a, (∀ a', R a' a → C a') → C a) (F' : ∀ a, (∀ a', R (f a') (f a) → C (f a')) → C (f a))
+    (h : ∀ a r, F (f a) r = F' a fun a' hR => r (f a') hR) (a : α') (h : WellFounded R) :
+    totalExtrinsicFix (C := (C <| f ·)) (InvImage R f) F' a = totalExtrinsicFix (C := C) R F (f a) := by
+  have h' := h
+  rcases h with ⟨h⟩
+  specialize h (f a)
+  have : Acc (InvImage R f) a := InvImage.accessible _ h
+  clear h
+  induction this
+  rename_i ih
+  rw [totalExtrinsicFix_eq_apply, totalExtrinsicFix_eq_apply, h]
+  · congr; ext a x
+    rw [ih _ x]
+  · assumption
+  · exact InvImage.wf _ ‹_›
+
+public theorem WellFounded.extrinsicFix_eq [∀ a, Nonempty (C a)] (R : α → α → Prop)
+    (F : ∀ a, (∀ a', R a' a → C a') → C a) (a : α) (h : Acc R a) :
+    extrinsicFix R F a = F a (fun a' _ => extrinsicFix R F a') := by
+  simp only [extrinsicFix]
+  rw [totalExtrinsicFix_eq_apply]
+  congr; ext a' hR
+  let f (x : { x : α // x = a' ∨ TransGen R x a' }) : { x : α // x = a ∨ TransGen R x a } :=
+    ⟨x.val, by
+      cases x.property
+      · rename_i h
+        rw [h]
+        exact Or.inr (.single hR)
+      · rename_i h
+        apply Or.inr
+        refine TransGen.trans h ?_
+        exact .single hR⟩
+  have := totalExtrinsicFix_invImage (C := (C ·.val)) (R := (R ·.1 ·.1)) (f := f)
+    (F := fun a r => F a.1 fun a' hR => r ⟨a', Or.inr (by rcases a.2 with ha | ha; exact .single (ha ▸ hR); exact .trans (.single hR) ‹_›)⟩ hR)
+    (F' := fun a r => F a.1 fun a' hR => r ⟨a', by rcases a.2 with ha | ha; exact .inr (.single (ha ▸ hR)); exact .inr (.trans (.single hR) ‹_›)⟩ hR)
+  unfold InvImage at this
+  rw [this]
+  · simp +zetaDelta
+  · constructor
+    intro x
+    refine InvImage.accessible _ ?_
+    cases x.2 <;> rename_i hx
+    · rwa [hx]
+    · exact h.invTransGen hx
+  · constructor
+    intro x
+    refine InvImage.accessible _ ?_
+    cases x.2 <;> rename_i hx
+    · rwa [hx]
+    · exact h.invTransGen hx
+
+@[inline]
+public def WellFounded.extrinsicFix₂ [∀ a b, Nonempty (C₂ a b)]
+    (R : (a : α) ×' β a → (a : α) ×' β a → Prop)
+    (F : (a : α) → (b : β a) → ((a' : α) → (b' : β a') → R ⟨a', b'⟩ ⟨a, b⟩ → C₂ a' b') → C₂ a b)
+    (a : α) (b : β a) :
+    C₂ a b :=
+  totalExtrinsicFix₂ (α := α) (β := fun a' => { b' : β a' // (PSigma.mk a' b') = (PSigma.mk a b) ∨ TransGen R ⟨a', b'⟩ ⟨a, b⟩ })
+      (C₂ := (C₂ · ·.1))
+      (fun p q => R ⟨p.1, p.2.1⟩ ⟨q.1, q.2.1⟩)
+      (fun a b recur => F a b.1 fun a' b' hR => recur a' ⟨b', Or.inr (by
+        rcases b.property with hb | hb
+        · exact .single (hb ▸ hR)
+        · apply TransGen.trans ?_ ‹_›
+          apply TransGen.single
+          assumption)⟩ ‹_›) a ⟨b, Or.inl rfl⟩
+
+public theorem WellFounded.extrinsicFix₂_eq_extrinsicFix [∀ a b, Nonempty (C₂ a b)]
+    (R : (a : α) ×' β a → (a : α) ×' β a → Prop)
+    (F : (a : α) → (b : β a) → ((a' : α) → (b' : β a') → R ⟨a', b'⟩ ⟨a, b⟩ → C₂ a' b') → C₂ a b)
+    (a : α) (b : β a) (h : Acc R ⟨a, b⟩) :
+    extrinsicFix₂ R F a b = extrinsicFix (α := PSigma β) (C := fun a => C₂ a.1 a.2) R (fun p r => F p.1 p.2 fun a' b' hR => r ⟨a', b'⟩ hR) ⟨a, b⟩ := by
+  simp only [extrinsicFix, extrinsicFix₂, totalExtrinsicFix₂]
+  let f (x : ((a' : α) ×' { b' // PSigma.mk a' b' = ⟨a, b⟩ ∨ TransGen R ⟨a', b'⟩ ⟨a, b⟩ })) : { a' // a' = ⟨a, b⟩ ∨ TransGen R a' ⟨a, b⟩ } :=
+    ⟨⟨x.1, x.2.1⟩, x.2.2⟩
+  have := totalExtrinsicFix_invImage (C := fun a => C₂ a.1.1 a.1.2) (f := f) (R := (R ·.1 ·.1))
+    (F := fun a r => F a.1.1 a.1.2 fun a' b' hR => r ⟨⟨a', b'⟩, ?refine_a⟩ hR)
+    (F' := fun a r => F a.1 a.2.1 fun a' b' hR => r ⟨a', b', ?refine_b⟩ hR)
+    (a := ⟨a, b, ?refine_c⟩); rotate_left
+  · cases a.2 <;> rename_i heq
+    · rw [heq] at hR
+      exact .inr (.single hR)
+    · exact .inr (.trans (.single hR) heq)
+  · cases a.2.2 <;> rename_i heq
+    · rw [heq] at hR
+      exact .inr (.single hR)
+    · exact .inr (.trans (.single hR) heq)
+  · exact .inl rfl
+  unfold InvImage f at this
+  simp at this
+  rw [this]
+  constructor
+  intro x
+  apply InvImage.accessible
+  cases x.2 <;> rename_i heq
+  · rwa [heq]
+  · exact h.invTransGen heq
+
+@[inline]
+public def WellFounded.extrinsicFix₃ [∀ a b c, Nonempty (C₃ a b c)]
+    (R : (a : α) ×' (b : β a) ×' γ a b → (a : α) ×' (b : β a) ×' γ a b → Prop)
+    (F : (a : α) → (b : β a) → (c : γ a b) → ((a' : α) → (b' : β a') → (c' : γ a' b') → R ⟨a', b', c'⟩ ⟨a, b, c⟩ → C₃ a' b' c') → C₃ a b c)
+    (a : α) (b : β a) (c : γ a b) :
+    C₃ a b c :=
+  totalExtrinsicFix₃ (α := α) (β := β) (γ := fun a' b' => { c' : γ a' b' // (⟨a', b', c'⟩ : (a : α) ×' (b : β a) ×' γ a b) = ⟨a, b, c⟩ ∨ TransGen R ⟨a', b', c'⟩ ⟨a, b, c⟩ })
+      (C₃ := (C₃ · · ·.1))
+      (fun p q => R ⟨p.1, p.2.1, p.2.2.1⟩ ⟨q.1, q.2.1, q.2.2.1⟩)
+      (fun a b c recur => F a b c.1 fun a' b' c' hR => recur a' b' ⟨c', Or.inr (by
+        rcases c.property with hb | hb
+        · exact .single (hb ▸ hR)
+        · apply TransGen.trans ?_ ‹_›
+          apply TransGen.single
+          assumption)⟩ ‹_›) a b ⟨c, Or.inl rfl⟩
+
+public theorem WellFounded.extrinsicFix₃_eq_extrinsicFix [∀ a b c, Nonempty (C₃ a b c)]
+    (R : (a : α) ×' (b : β a) ×' γ a b → (a : α) ×' (b : β a) ×' γ a b → Prop)
+    (F : (a : α) → (b : β a) → (c : γ a b) → ((a' : α) → (b' : β a') → (c' : γ a' b') → R ⟨a', b', c'⟩ ⟨a, b, c⟩ → C₃ a' b' c') → C₃ a b c)
+    (a : α) (b : β a) (c : γ a b) (h : Acc R ⟨a, b, c⟩) :
+    extrinsicFix₃ R F a b c = extrinsicFix (α := (a : α) ×' (b : β a) ×' γ a b) (C := fun a => C₃ a.1 a.2.1 a.2.2) R (fun p r => F p.1 p.2.1 p.2.2 fun a' b' c' hR => r ⟨a', b', c'⟩ hR) ⟨a, b, c⟩ := by
+  simp only [extrinsicFix, extrinsicFix₃, totalExtrinsicFix₃]
+  let f (x : ((a' : α) ×' (b' : β a') ×' { c' // (⟨a', b', c'⟩ : (a : α) ×' (b : β a) ×' γ a b) = ⟨a, b, c⟩ ∨ TransGen R ⟨a', b', c'⟩ ⟨a, b, c⟩ })) : { a' // a' = ⟨a, b, c⟩ ∨ TransGen R a' ⟨a, b, c⟩ } :=
+    ⟨⟨x.1, x.2.1, x.2.2.1⟩, x.2.2.2⟩
+  have := totalExtrinsicFix_invImage (C := fun a => C₃ a.1.1 a.1.2.1 a.1.2.2) (f := f) (R := (R ·.1 ·.1))
+    (F := fun a r => F a.1.1 a.1.2.1 a.1.2.2 fun a' b' c' hR => r ⟨⟨a', b', c'⟩, ?refine_a⟩ hR)
+    (F' := fun a r => F a.1 a.2.1 a.2.2.1 fun a' b' c' hR => r ⟨a', b', c', ?refine_b⟩ hR)
+    (a := ⟨a, b, c, ?refine_c⟩); rotate_left
+  · cases a.2 <;> rename_i heq
+    · rw [heq] at hR
+      exact .inr (.single hR)
+    · exact .inr (.trans (.single hR) heq)
+  · cases a.2.2.2 <;> rename_i heq
+    · rw [heq] at hR
+      exact .inr (.single hR)
+    · exact .inr (.trans (.single hR) heq)
+  · exact .inl rfl
+  unfold InvImage f at this
+  simp at this
+  rw [this]
+  constructor
+  intro x
+  apply InvImage.accessible
+  cases x.2 <;> rename_i heq
+  · rwa [heq]
+  · exact h.invTransGen heq
 
 end WellFounded
